correctness/RegexCorrectness/Strategy/Materialize/Basic.lean
@@ -3,7 +3,7 @@ import RegexCorrectness.Data.Expr.Semantics.CaptureGroups
 set_option autoImplicit false
 
 open Regex.Data (CaptureGroups)
-open String (Pos)
+open String.Pos (Raw)
 
 namespace Regex.Strategy
 
@@ -11,7 +11,7 @@ namespace Regex.Strategy
 `materializeRegexGroups groups` constructs a mapping that associates each capture group's tag
 with the start/end positions of the last appearance of the capture group in the input string.
 -/
-def materializeRegexGroups : CaptureGroups → Nat → Option (Pos × Pos)
+def materializeRegexGroups : CaptureGroups → Nat → Option (Raw × Raw)
   | .empty, _ => .none
   | .group tag first last groups, tag' =>
     if tag = tag' then
@@ -22,7 +22,7 @@ def materializeRegexGroups : CaptureGroups → Nat → Option (Pos × Pos)
     -- The later one will be preferred
     materializeRegexGroups g₂ tag <|> materializeRegexGroups g₁ tag
 
-def materializeUpdatesAux (n : Nat) (accum : Vector (Option Pos) n) : List (Nat × Pos) → Vector (Option Pos) n
+def materializeUpdatesAux (n : Nat) (accum : Vector (Option Raw) n) : List (Nat × Raw) → Vector (Option Raw) n
   | [] => accum
   | (offset, pos) :: rest =>
     materializeUpdatesAux n (accum.setIfInBounds offset (some pos)) rest
@@ -32,16 +32,16 @@ def materializeUpdatesAux (n : Nat) (accum : Vector (Option Pos) n) : List (Nat 
 as the writes to the buffer. When the same offset appears multiple times in the list, the last
 one wins.
 -/
-def materializeUpdates (n : Nat) (updates : List (Nat × Pos)) : Vector (Option Pos) n :=
+def materializeUpdates (n : Nat) (updates : List (Nat × Raw)) : Vector (Option Raw) n :=
   materializeUpdatesAux n (Vector.replicate n .none) updates
 
-def EquivMaterializedUpdate {n} (groups : Nat → Option (Pos × Pos)) (updates : Vector (Option Pos) n) : Prop :=
+def EquivMaterializedUpdate {n} (groups : Nat → Option (Raw × Raw)) (updates : Vector (Option Raw) n) : Prop :=
   ∀ tag,
     ((h₁ : 2 * tag < n) → ((groups tag).map (·.1) = updates[2 * tag])) ∧
     ((h₂ : 2 * tag + 1 < n) → ((groups tag).map (·.2) = updates[2 * tag + 1]))
 
-theorem EquivMaterializedUpdate.eq {n} {groups : Nat → Option (Pos × Pos)} {updates : Vector (Option Pos) n}
-  (eqv : EquivMaterializedUpdate groups updates) (tag : Nat) (lt : 2 * tag + 1 < n) (p₁ p₂ : Pos) :
+theorem EquivMaterializedUpdate.eq {n} {groups : Nat → Option (Raw × Raw)} {updates : Vector (Option Raw) n}
+  (eqv : EquivMaterializedUpdate groups updates) (tag : Nat) (lt : 2 * tag + 1 < n) (p₁ p₂ : Raw) :
   groups tag = .some (p₁, p₂) ↔ updates[2 * tag] = .some p₁ ∧ updates[2 * tag + 1] = .some p₂ := by
   have eq₁ := (eqv tag).1 (by omega)
   have eq₂ := (eqv tag).2 lt
