regex/Regex/Data/String.lean
@@ -1,35 +1,71 @@
 namespace String
 
-@[simp]
-theorem utf8Size.go_append (cs₁ cs₂ : List Char) : utf8ByteSize.go (cs₁ ++ cs₂) = utf8ByteSize.go cs₁ + utf8ByteSize.go cs₂ := by
-  induction cs₁ with
-  | nil => simp [utf8ByteSize.go]
-  | cons c cs₁ ih =>
-    simp [utf8ByteSize.go, ih]
-    omega
+theorem _root_.List.asString_cons {c : Char} {cs : List Char} :
+  (c :: cs).asString = [c].asString ++ cs.asString := by
+  simp [←List.asString_append]
 
-@[simp]
-theorem utf8Size.go_nil : utf8ByteSize.go [] = 0 := rfl
+theorem Pos.Raw.utf8GetAux_utf8Size_le_utf8Encode_size (cs₁ cs₂ cs₃ : List Char) (i p : Pos.Raw)
+  (eq₁ : i = cs₁.asString.endPos) (eq₂ : p = (cs₁ ++ cs₂).asString.endPos) (lt : 0 < cs₃.length) (v : p.IsValid (cs₁ ++ cs₂ ++ cs₃).asString) :
+  (Pos.Raw.utf8GetAux (cs₂ ++ cs₃) i p).utf8Size ≤ cs₃.asString.utf8ByteSize := by
+  match cs₂, cs₃, lt with
+  | [], c :: cs₃, _ =>
+    simp only [List.append_nil] at eq₂
+    simp only [← eq₂] at eq₁
+    simp only [List.nil_append, eq₁, utf8GetAux, ↓reduceIte, ge_iff_le]
+    rw [List.asString_cons, String.utf8ByteSize_append, ←String.singleton_eq, String.utf8ByteSize_singleton]
+    exact Nat.le_add_right _ _
+  | c :: cs₂, cs₃, lt =>
+    have ne : i ≠ p := by
+      refine Pos.Raw.ne_of_lt ?_
+      simp only [eq₁, endPos, eq₂, List.asString_append, utf8ByteSize_append, mk_lt_mk, Nat.lt_add_right_iff_pos]
+      rw [List.asString_cons, String.utf8ByteSize_append, ←String.singleton_eq, String.utf8ByteSize_singleton]
+      exact Nat.lt_of_lt_of_le c.utf8Size_pos (by grind)
+    simp only [List.cons_append, utf8GetAux, ne, ↓reduceIte, ge_iff_le]
+    exact utf8GetAux_utf8Size_le_utf8Encode_size (cs₁ ++ [c]) cs₂ cs₃ (i + c) p (by simp [eq₁, endPos, ←String.singleton_eq, Pos.Raw.ext_iff]) (by simpa using eq₂) lt (by simpa using v)
 
-@[simp]
-theorem utf8Size.go_cons (c : Char) (cs : List Char) : utf8ByteSize.go (c :: cs) = utf8ByteSize.go cs + c.utf8Size := by
-  simp [utf8ByteSize.go]
+theorem Pos.Raw.next_le_endPos {s : String} {p : Pos.Raw} (v : p.IsValid s) (h : p ≠ s.endPos) : p.next s ≤ s.endPos := by
+  have ⟨m₁, m₂, eq₁, eq₂⟩ := Pos.Raw.isValid_iff_exists_append.mp v
+  have lt : 0 < m₂.length := by
+    apply Nat.zero_lt_of_ne_zero
+    intro eq
+    have eq' : m₂ = "" := String.data_eq_nil_iff.mp (List.eq_nil_iff_length_eq_zero.mpr (by simpa using eq))
+    simp_all
+  have le := Pos.Raw.utf8GetAux_utf8Size_le_utf8Encode_size [] m₁.data m₂.data 0 p rfl (by simpa using eq₂) lt (by simpa [←eq₁] using v)
+  have eq : (utf8GetAux (m₁.data ++ m₂.data) 0 p) = p.get s := by
+    congr
+    simp [eq₁]
+  rw [eq] at le
+  simp only [next, le_iff, byteIdx_add_char, byteIdx_endPos, ge_iff_le]
+  calc p.byteIdx + (get s p).utf8Size
+    _ ≤ p.byteIdx + m₂.data.asString.utf8ByteSize := by grind
+    _ ≤ m₁.endPos.byteIdx + m₂.data.asString.utf8ByteSize := by grind
+    _ ≤ s.utf8ByteSize := by simp [eq₁]
 
-theorem next_le_endPosAux (p : Pos) (cs : List Char) (i ep : Pos) (lt : p < ep) (hep : ep = i + ⟨utf8ByteSize.go cs⟩) : p + utf8GetAux cs i p ≤ ep := by
-  induction cs generalizing i with
-  | nil =>
-    simp [utf8GetAux, hep] at *
-    exact Nat.succ_le_of_lt lt
-  | cons c cs ih =>
-    simp [utf8GetAux]
-    split
-    next eq =>
-      rw [hep, eq]
-      exact Nat.add_le_add_left (by simp) p.byteIdx
-    next ne => exact ih (i + c) (by simp [hep, Pos.ext_iff, Nat.add_assoc, Nat.add_comm])
+theorem Pos.Raw.utf8GetAux_eq_default_of_not_valid (cs₁ cs₂ : List Char) (i p : Pos.Raw)
+  (eq : i = cs₁.asString.endPos)
+  (h : i.IsValid (cs₁ ++ cs₂).asString) (h' : ¬p.IsValid (cs₁ ++ cs₂).asString) :
+  Pos.Raw.utf8GetAux cs₂ i p = default := by
+  fun_induction Pos.Raw.utf8GetAux generalizing cs₁
+  next => rfl
+  next => grind
+  next c cs₂ i p ne ih =>
+    have eq' : i + c = (cs₁ ++ [c]).asString.endPos := by
+      simp [eq, String.endPos, Pos.Raw.ext_iff, ←String.singleton_eq_asString]
+    have h : IsValid (cs₁ ++ [c] ++ cs₂).asString (i + c) := by
+      rw [Pos.Raw.isValid_iff_exists_append]
+      exists (cs₁ ++ [c]).asString, cs₂.asString
+      refine ⟨List.asString_append, ?_⟩
+      simp [eq, ←String.singleton_eq_asString, String.endPos, Pos.Raw.ext_iff]
+    exact ih (cs₁ ++ [c]) eq' h (by simpa using h')
 
-theorem next_le_endPos (s : String) (p : Pos) (lt : p < s.endPos) : s.next p ≤ s.endPos :=
-  next_le_endPosAux p s.data 0 s.endPos lt (by simp [String.endPos, String.utf8ByteSize, Pos.ext_iff])
+theorem Pos.Raw.get_eq_default_of_not_valid {p : Pos.Raw} {s : String} (h : ¬p.IsValid s) : p.get s = default :=
+  Pos.Raw.utf8GetAux_eq_default_of_not_valid [] s.data 0 p rfl Pos.Raw.isValid_zero (by simpa using h)
+
+theorem next_le_endPos (s : String) (p : Pos.Raw) (lt : p < s.endPos) : p.next s ≤ s.endPos := by
+  if v : p.IsValid s then
+    exact Pos.Raw.next_le_endPos v (ne_of_apply_ne Pos.Raw.byteIdx (Nat.ne_of_lt lt))
+  else
+    simpa [Pos.Raw.next, Pos.Raw.get_eq_default_of_not_valid v] using Nat.succ_le_of_lt lt
 
 end String
 
@@ -71,19 +107,19 @@ theorem next_le_endPos (it : Iterator) (h : it.hasNext) : (it.next' h).pos ≤ (
 
 theorem lt_next (it : Iterator) : it.pos < it.next.pos := by
   simp [pos, next]
-  exact String.lt_next _ _
+  exact String.Pos.Raw.byteIdx_lt_byteIdx_next _ _
 
-theorem next_le_four (it : Iterator) : it.next.pos ≤ it.pos + ⟨4⟩ := by
-  simp [pos, next, String.next]
-  show it.pos.byteIdx + Char.utf8Size (it.toString.get it.pos) ≤ it.pos.byteIdx + 4
+theorem next_le_four (it : Iterator) : it.next.pos.byteIdx ≤ it.pos.byteIdx + 4 := by
+  show it.pos.byteIdx + Char.utf8Size (it.pos.get it.toString) ≤ it.pos.byteIdx + 4
   simp [Char.utf8Size_le_four]
 
 @[simp]
 theorem next'_remainingBytes_lt {it : Iterator} {h : it.hasNext} : (it.next' h).remainingBytes < it.remainingBytes := by
-  simp [hasNext] at h
-  simp [next', remainingBytes, String.next]
-  have : (it.s.get it.i).utf8Size > 0 := Char.utf8Size_pos _
-  omega
+  simp only [hasNext, byteIdx_endPos, decide_eq_true_eq] at h
+  simp only [remainingBytes, next', Pos.Raw.next'_eq, Pos.Raw.next, byteIdx_endPos,
+    Pos.Raw.byteIdx_add_char]
+  have : (Pos.Raw.get it.s it.i).utf8Size > 0 := Char.utf8Size_pos _
+  grind
 
 theorem curr'_eq_curr {it : Iterator} {h : it.hasNext} : it.curr' h = it.curr := by
   simp [curr', curr]
